complexity proof for indcpa-1 indcpa-n almost finish

theories/encryption/PKE_hybrid.ec
@@ -8,6 +8,8 @@
 
 require import AllCore List FSet Finite Distr OldMonoid.
 require import Indist.
+require (*--*) CHoareTactic.
+(*---*) import StdBigop.Bigint BIA.
 
 type pkey.
 type skey.
@@ -43,7 +45,6 @@ module type AdvCPA(LR:LR) = {
 }.
 
 module K = {
-  var c  : int
   var pk : pkey
   var sk : skey
   var b  : bool
@@ -54,7 +55,6 @@ module L (S:Scheme) = {
   proc orcl (m0 m1:plaintext) : ciphertext = {
     var r : ciphertext;
     r   <@ S.enc(K.pk,m0);
-    K.c <- K.c + 1;
     return r;
   }
 }.
@@ -64,7 +64,6 @@ module R (S:Scheme) = {
   proc orcl (m0 m1:plaintext) : ciphertext = {
     var r : ciphertext;
     r   <@ S.enc(K.pk,m1);
-    K.c <- K.c + 1;
     return r;
   }
 }.
@@ -74,7 +73,6 @@ module LRb (S:Scheme) = {
   proc orcl (m0 m1:plaintext) : ciphertext = {
     var r : ciphertext;
     r   <@ S.enc(K.pk,K.b?m0:m1);
-    K.c <- K.c + 1;
     return r;
   }
 }.
@@ -83,7 +81,6 @@ module CPAL (S:Scheme,A:AdvCPA) = {
   module A = A(L(S))
   proc main():bool = {
     var b':bool;
-    K.c         <- 0;
     (K.pk,K.sk) <@ S.kg();
     b'          <@ A.main(K.pk);
     return b';
@@ -94,7 +91,6 @@ module CPAR (S:Scheme,A:AdvCPA) = {
   module A = A(R(S))
   proc main():bool = {
     var b':bool;
-    K.c         <- 0;
     (K.pk,K.sk) <@ S.kg();
     b'          <@ A.main(K.pk);
     return b';
@@ -105,7 +101,6 @@ module CPA (S:Scheme,A:AdvCPA) = {
   module A = A(LRb(S))
   proc main():bool = {
     var b':bool;
-    K.c         <- 0;
     K.b         <$ {0,1};
     (K.pk,K.sk) <@ S.kg();
     b'          <@ A.main(K.pk);
@@ -132,12 +127,11 @@ module ToOrcl (S:Scheme) = {
 }.
 
 module ToAdv(A:AdvCPA, O:Orcl,LR:LR) = {
-  module A = A(LR)
   proc main() : bool = {
     var pk:pkey;
     var b':bool;
     pk <@ O.leaks();
-    b' <@ A.main(pk);
+    b' <@ A(LR).main(pk);
     return b';
   }
 }.
@@ -153,82 +147,304 @@ module B (S:Scheme, A:AdvCPA, LR:LR) = {
   }
 }.
 
+(* Complexity of the adversary *)
+op cA : { int | 0 <= cA } as cA_pos.
+
+type cScheme = {
+  ckg  : int;
+  cenc : int;
+  cdec : int;
+}.
+
+(* Complexity of the scheme *)
+op cs : cScheme.
+axiom cs_pos : 0 <= cs.`ckg /\ 0 <= cs.`cenc /\ 0 <= cs.`cdec.
+
+op cincr : int -> int.
+schema cost_incr {n:int} (m:int) : cost[`|n| <= m : n + 1] = cost[true:n] + cincr m.
+hint simplify cost_incr.
+
+op cltint : int -> int.
+schema cost_ltint {n1 n2:int} (m:int) : cost[`|n1| <= m /\ `|n2| <= m : n1 < n2] = cost[true:n1] + cost[true:n2] + cltint m.
+hint simplify cost_ltint.
+
+op ceqint : int -> int.
+schema cost_eqint {n1 n2:int} (m:int) : cost[`|n1| <= m /\ `|n2| <= m : n1 = n2] = cost[true:n1] + cost[true:n2] + ceqint m.
+hint simplify cost_eqint.
+
+schema cost_ltint_P `{P} {n1 n2:int} (m:int) : cost[P /\ `|n1| <= m /\ `|n2| <= m : n1 < n2] = cost[P:n1] + cost[P:n2] + cltint m.
+hint simplify cost_ltint_P.
+
+schema cost_eqint_P `{P} {n1 n2:int} (m:int) : cost[P /\ `|n1| <= m /\ `|n2| <= m : n1 = n2] = cost[P:n1] + cost[P:n2] + ceqint m.
+hint simplify cost_eqint_P.
+
+op cdinterval : int -> int.
+schema cost_dinterval {i j : int} (k:int) : cost [ i <= j <= k - i : [i .. j - 1]] = cost [true : i] + cost [true : j] + cdinterval k.
+hint simplify cost_dinterval.
+
+axiom ge0_cincr m : 0 <= cincr m.
+axiom ge0_cltint m : 0 <= cltint m.
+axiom ge0_ceqint m : 0 <= ceqint m.
+axiom ge0_cdinterval m : 0 <= cdinterval m.
+
+(* FIXME : does it make sense ? *)
+schema cost_Hq `{P} : cost [P : H.q] = 0.
+hint simplify cost_Hq.
+
 section.
 
-  declare module S:Scheme {-K, -H.Count, -H.HybOrcl}.
+  declare module S:Scheme [ kg : `{cs.`ckg},
+                            enc: `{cs.`cenc}]
+                 {-K, -H.Count, -H.HybOrcl}.
     (* Normaly I would like to locally
        clone Indist in the section, in that case
        restrictions at least on H.c are not needed.
        But LRB and B are used so we need to do it
      *)
+  
+  declare module A:AdvCPA [main : `{cA, #LR.orcl: H.q}] {-K,-H.Count,-H.HybOrcl,-S}.
 
-  declare module A:AdvCPA {-K,-H.Count,-H.HybOrcl,-S}.
-
-  axiom Lkg  : islossless S.kg.
-  axiom Lenc : islossless S.enc.
   axiom La   : forall (LR<:LR{-A}), islossless LR.orcl => islossless A(LR).main.
 
-  lemma CPA1_CPAn &m : 0 < H.q =>
-    Pr[CPAL(S,B(S,A)).main() @ &m : res /\ H.HybOrcl.l <= H.q /\ K.c <= 1] -
-    Pr[CPAR(S,B(S,A)).main() @ &m : res /\ H.HybOrcl.l <= H.q /\ K.c <= 1] =
-    1%r/H.q%r * (Pr[CPAL(S,A).main() @ &m : res /\ K.c <= H.q] -
-                 Pr[CPAR(S,A).main() @ &m : res /\ K.c <= H.q]).
+  local lemma cost_AL : 
+     choare [A(OrclL(ToOrcl(S))).main : H.Count.c = 0 ==> H.Count.c <= H.q] 
+     time [cincr H.q * H.q;
+           A.main : 1;
+           S.enc  : H.q].
   proof.
-    move=> Hq.
-    cut -> : Pr[CPAL(S, A).main() @ &m : res /\ K.c <= H.q] =
-             Pr[INDL(ToOrcl(S),ToAdv(A)).main() @ &m : res /\ H.Count.c <= H.q].
+    proc true :
+         (OrclL(ToOrcl(S)).orcl : H.Count.c) time
+         [ (OrclL(ToOrcl(S)).orcl : [fun _ => cincr H.q; S.enc : fun _ => 1]) ] => //.
+    + by move => />; rewrite !bigi_constz 1..2:[smt (H.q_pos)].
+    move=> zo hzo; proc; inline *; wp := (`|H.Count.c| <= H.q); call (: true); auto => &hr /> /#.
+  qed.
+
+  local lemma AL_bound : hoare [A(OrclL(ToOrcl(S))).main : H.Count.c = 0 ==> H.Count.c <= H.q].
+  proof. by conseq cost_AL. qed.
+
+  local lemma cost_AR : 
+     choare [A(OrclR(ToOrcl(S))).main : H.Count.c = 0 ==> H.Count.c <= H.q] 
+     time [cincr H.q * H.q;
+           A.main : 1;
+           S.enc  : H.q].
+  proof.
+    proc true :
+         (OrclR(ToOrcl(S)).orcl : H.Count.c) time
+         [ (OrclR(ToOrcl(S)).orcl : [fun _ => cincr H.q; S.enc : fun _ => 1]) ] => //.
+    + by move => />; rewrite !bigi_constz 1..2:[smt (H.q_pos)].
+    move=> zo hzo; proc; inline *; wp; call(:true); wp:=(`|H.Count.c| <= H.q); skip => &hr /> /#.
+  qed.
+
+  local lemma AR_bound : hoare [A(OrclR(ToOrcl(S))).main : H.Count.c = 0 ==> H.Count.c <= H.q].
+  proof. by conseq cost_AR. qed.
+
+  local lemma cost_AHL : 
+     choare [A(HybOrcl2(ToOrcl(S), OrclL(ToOrcl(S)))).main : 
+         0 <= H.HybOrcl.l0 <= H.q /\ H.HybOrcl.l = 0 /\ H.Count.c = 0 ==> 
+         H.HybOrcl.l <= H.q /\ H.Count.c <= 1 ]
+      time [(cincr H.q + cincr 1 + cltint H.q + ceqint H.q) * H.q; S.enc : H.q; A.main : 1].
+  proof.
+    proc 
+      (0 <= H.HybOrcl.l /\ 0 <= H.HybOrcl.l0 <= H.q /\ H.Count.c = if H.HybOrcl.l <= H.HybOrcl.l0 then 0 else 1):
+      (HybOrcl2(ToOrcl(S), OrclL(ToOrcl(S))).orcl :  H.HybOrcl.l) time
+      [ (HybOrcl2(ToOrcl(S), OrclL(ToOrcl(S))).orcl : [fun _ => cincr H.q + cincr 1 + cltint H.q + ceqint H.q; S.enc : fun _ => 1]) ] => //=.
+    + by rewrite !bigi_constz 1,2:[smt(H.q_pos)].
+    + by move=> &hr /> ->.
+    + by move=> /> /#.
+    move=> zo hzo; proc; inline *.
+    wp := (`|H.HybOrcl.l| <= H.q).
+    if := (`| H.HybOrcl.l0| <= H.q /\ `|H.HybOrcl.l| <= H.q); 1: smt().
+    + by wp; call (:true; time []); auto => &hr />; smt (ge0_cincr ge0_cltint ge0_ceqint).
+    if := (`| H.HybOrcl.l0| <= H.q /\ `|H.HybOrcl.l| <= H.q); 1: smt().
+    + wp := (`|H.Count.c| <= 1); call (:true; time []); auto => &hr />.
+      smt (ge0_cincr ge0_cltint ge0_ceqint).
+    by wp; call (:true; time []); auto => &hr />; smt (ge0_cincr ge0_cltint ge0_ceqint).
+  qed.
+
+  local lemma AHL_bound :  
+     hoare [A(HybOrcl2(ToOrcl(S), OrclL(ToOrcl(S)))).main : 
+         0 <= H.HybOrcl.l0 <= H.q /\ H.HybOrcl.l = 0 /\ H.Count.c = 0 ==> 
+         H.HybOrcl.l <= H.q /\ H.Count.c <= 1 ].
+  proof. by conseq cost_AHL. qed.
+
+  local lemma cost_AHR : 
+     choare [A(HybOrcl2(ToOrcl(S), OrclR(ToOrcl(S)))).main : 
+         0 <= H.HybOrcl.l0 <= H.q /\ H.HybOrcl.l = 0 /\ H.Count.c = 0 ==> 
+         H.HybOrcl.l <= H.q /\ H.Count.c <= 1 ]
+      time [(cincr H.q + cincr 1 + cltint H.q + ceqint H.q) * H.q; S.enc : H.q; A.main : 1].
+  proof.
+    proc 
+      (0 <= H.HybOrcl.l /\ 0 <= H.HybOrcl.l0 <= H.q /\ H.Count.c = if H.HybOrcl.l <= H.HybOrcl.l0 then 0 else 1):
+      (HybOrcl2(ToOrcl(S), OrclR(ToOrcl(S))).orcl :  H.HybOrcl.l) time
+      [ (HybOrcl2(ToOrcl(S), OrclR(ToOrcl(S))).orcl : [fun _ => cincr H.q + cincr 1 + cltint H.q + ceqint H.q; S.enc : fun _ => 1]) ] => //=.
+    + by rewrite !bigi_constz 1,2:[smt(H.q_pos)].
+    + by move=> &hr /> ->.
+    + by move=> /> /#.
+    move=> zo hzo; proc; inline *.
+    wp := (`|H.HybOrcl.l| <= H.q).
+    if := (`| H.HybOrcl.l0| <= H.q /\ `|H.HybOrcl.l| <= H.q); 1: smt().
+    + by wp; call (:true; time []); auto => &hr />; smt (ge0_cincr ge0_cltint ge0_ceqint).
+    if := (`| H.HybOrcl.l0| <= H.q /\ `|H.HybOrcl.l| <= H.q); 1: smt().
+    + wp; call (:true; time []); wp := (`|H.Count.c| <= 1); skip => &hr />.
+      smt (ge0_cincr ge0_cltint ge0_ceqint).
+    by wp; call (:true; time []); auto => &hr />; smt (ge0_cincr ge0_cltint ge0_ceqint).
+  qed.
+
+  local lemma AHR_bound :  
+     hoare [A(HybOrcl2(ToOrcl(S), OrclR(ToOrcl(S)))).main : 
+         0 <= H.HybOrcl.l0 <= H.q /\ H.HybOrcl.l = 0 /\ H.Count.c = 0 ==> 
+         H.HybOrcl.l <= H.q /\ H.Count.c <= 1 ].
+  proof. by conseq cost_AHR. qed.
+ 
+  lemma CPA1_CPAn &m :
+    Pr[CPAL(S,B(S,A)).main() @ &m : res] -
+    Pr[CPAR(S,B(S,A)).main() @ &m : res] =
+    1%r/H.q%r * (Pr[CPAL(S,A).main() @ &m : res] - Pr[CPAR(S,A).main() @ &m : res]).
+  proof.
+    cut -> : Pr[CPAL(S, A).main() @ &m : res] =
+             Pr[INDL(ToOrcl(S),ToAdv(A)).main() @ &m : res].
       byequiv (_ : ={glob A, glob S} ==>
-                        ={res,glob A, glob S, K.pk} /\ K.c{1} = H.Count.c{2}) => //.
+                        ={res,glob A, glob S, K.pk}) => //.
       proc.
       inline INDL(ToOrcl(S), ToAdv(A)).A.main H.Count.init  ToOrcl(S).leaks.
-      wp;call (_: ={glob S, K.pk} /\ K.c{1} = H.Count.c{2}).
+      wp;call (_: ={glob S, K.pk}).
         by proc;inline ToOrcl(S).orcl H.Count.incr;wp;call (_:true);wp.
       by wp;call (_:true);wp.
-    cut -> : Pr[CPAR(S, A).main() @ &m : res /\ K.c <= H.q] =
-             Pr[INDR(ToOrcl(S),ToAdv(A)).main() @ &m : res /\ H.Count.c <= H.q].
+    cut -> : Pr[CPAR(S, A).main() @ &m : res] =
+             Pr[INDR(ToOrcl(S),ToAdv(A)).main() @ &m : res].
       byequiv (_ : ={glob A, glob S} ==>
-                        ={res,glob A, glob S, K.pk} /\ K.c{1} = H.Count.c{2}) => //.
+                        ={res,glob A, glob S, K.pk}) => //.
       proc.
       inline INDR(ToOrcl(S), ToAdv(A)).A.main H.Count.init  ToOrcl(S).leaks.
-      wp;call (_: ={glob S, K.pk} /\ K.c{1} = H.Count.c{2}).
+      wp;call (_: ={glob S, K.pk}).
         by proc;inline ToOrcl(S).orcl H.Count.incr;wp;call (_:true);wp.
       by wp;call (_:true);wp.
-    cut := IND1_INDn (ToOrcl(S)) (ToAdv(A)) _ _ _ _ &m (fun ga go c, true) => //=.
-      by proc;call Lkg.
-      by proc;call Lenc.
+    cut := IND1_INDn (ToOrcl(S)) (ToAdv(A)) _ _ _ H.q_pos &m (fun ga go c, true) => //=.
+    + have h : choare [ToOrcl(S).leaks : true ==> true] time [0; S.kg:1].
+      + by proc; call (_:true); skip.
+      conseq h.
+    + have h : choare [ToOrcl(S).orcl : true ==> true] time [0; S.enc:1].
+      + by proc; call (_:true); skip.
+      conseq h.
       move=> O LR Llr Ll Lo;proc;call (La LR _) => //.
       by call Ll.
+    have -> : Pr[INDL(ToOrcl(S), ToAdv(A)).main() @ &m : res /\ H.Count.c <= H.q] =
+              Pr[INDL(ToOrcl(S), ToAdv(A)).main() @ &m : res].
+    + byequiv => //.
+      conseq (_: ={glob A,glob S} ==> ={res}) (_: true ==> H.Count.c <= H.q) => //; last by sim.
+      proc; inline *; wp. by call AL_bound; wp; call (:true); wp.
+    have -> : Pr[INDR(ToOrcl(S), ToAdv(A)).main() @ &m : res /\ H.Count.c <= H.q] =
+              Pr[INDR(ToOrcl(S), ToAdv(A)).main() @ &m : res].
+    + byequiv => //.
+      conseq (_: ={glob A,glob S} ==> ={res}) (_: true ==> H.Count.c <= H.q) => //; last by sim.
+      by proc; inline *; wp; call AR_bound; wp; call(:true); auto.
     move=> <-; congr; last congr.
-      byequiv (_: ={glob S,glob A} ==> ={res,glob H.HybOrcl} /\ K.c{1} = H.Count.c{2}) => //.
+    + have -> : Pr[INDL(ToOrcl(S), HybGame2(ToAdv(A))).main() @ &m : res /\ H.HybOrcl.l <= H.q /\ H.Count.c <= 1] =
+                Pr[INDL(ToOrcl(S), HybGame2(ToAdv(A))).main() @ &m : res ].
+      + byequiv => //.
+        conseq (_: ={glob A,glob S} ==> ={res}) (_: true ==>  H.HybOrcl.l <= H.q /\ H.Count.c <= 1) => //; last by sim.
+        proc; inline *; wp; call AHL_bound; auto; call(:true); auto.
+        smt (DInterval.supp_dinter).
+      byequiv (_: ={glob S,glob A} ==> ={res,glob H.HybOrcl}) => //.
       proc.
       inline INDL(ToOrcl(S), Ind.HybGame2(ToAdv(A))).A.main H.Count.init CPAL(S, B(S,A)).A.main
         Ind.HybGame2(ToAdv(A), ToOrcl(S), OrclL(ToOrcl(S))).A.main.
       wp.
-      call (_: ={glob S,glob H.HybOrcl, K.pk} /\ K.c{1} = H.Count.c{2}).
+      call (_: ={glob S,glob H.HybOrcl, K.pk}).
         proc;wp.
         if => //.
           by call (_: ={glob S, K.pk});first sim.
         if => //.
-          call (_: ={glob S, K.pk} /\ K.c{1} = H.Count.c{2}) => //.
+          call (_: ={glob S, K.pk}) => //.
           by inline ToOrcl(S).orcl H.Count.incr;wp;call (_: true);wp.
         by call (_: ={glob S, K.pk});first sim.
-      swap{1} [4..5] -2;inline ToOrcl(S).leaks;wp.
+      swap{1} [3..4] -2;inline ToOrcl(S).leaks;wp.
       by call (_:true);wp;rnd;wp.
-    byequiv (_: ={glob S,glob A} ==> ={res,glob H.HybOrcl} /\ K.c{1} = H.Count.c{2}) => //.
+    have -> : Pr[INDR(ToOrcl(S), HybGame2(ToAdv(A))).main() @ &m : res /\ H.HybOrcl.l <= H.q /\ H.Count.c <= 1] =
+              Pr[INDR(ToOrcl(S), HybGame2(ToAdv(A))).main() @ &m : res].
+    + byequiv => //.
+      conseq (_: ={glob A,glob S} ==> ={res}) (_: true ==>  H.HybOrcl.l <= H.q /\ H.Count.c <= 1) => //; last by sim.
+      proc; inline *; wp; call AHR_bound; auto; call(:true); auto.
+      smt (DInterval.supp_dinter).
+    byequiv (_: ={glob S,glob A} ==> ={res,glob H.HybOrcl}) => //.
     proc.
     inline INDR(ToOrcl(S), Ind.HybGame2(ToAdv(A))).A.main H.Count.init CPAR(S, B(S,A)).A.main
       Ind.HybGame2(ToAdv(A), ToOrcl(S), OrclR(ToOrcl(S))).A.main.
-    wp.
-    call (_: ={glob S,glob H.HybOrcl, K.pk} /\ K.c{1} = H.Count.c{2}).
+    wp. 
+    call (_: ={glob S,glob H.HybOrcl, K.pk}).
       proc;wp.
       if => //.
         by call (_: ={glob S, K.pk});first sim.
       if => //.
-        call (_: ={glob S, K.pk} /\ K.c{1} = H.Count.c{2}) => //.
+        call (_: ={glob S, K.pk}) => //.
         by inline ToOrcl(S).orcl H.Count.incr;wp;call (_: true);wp.
       by call (_: ={glob S, K.pk});first sim.
-    swap{1} [4..5] -2;inline ToOrcl(S).leaks;wp.
+    swap{1} [3..4] -2;inline ToOrcl(S).leaks;wp.
     by call (_:true);wp;rnd;wp.
   qed.
+
+  lemma big_b2i ['a] (P:'a -> bool) s : big predT (fun k => b2i (P k)) s = big P (fun _ => 1) s.
+  proof. by rewrite (big_mkcond P); apply congr_big. qed.
+
+  lemma bigi_b2i_split (k n m:int) P F:
+    n <= k < m =>
+    bigi P F n m = bigi P F n k + b2i (P k) * F k + bigi P F (k+1) m.
+  proof.
+    move=> h; rewrite (big_cat_int k n m) 1,2:/#.
+    rewrite (big_ltn_cond k m) 1:/# /b2i; case: (P k) => *; ring.
+  qed.
+
+  lemma bigi_inP (n m:int) P F:
+    (forall i, n <= i < m => P i) =>
+    bigi P F n m = bigi predT F n m.
+  proof. by move=> h; apply congr_big_int => // i /h ->. qed.
+
+  lemma bigi1 (n m:int) P F:
+    (forall i, n <= i < m => P i => F i = 0) =>
+    bigi P F n m = 0.
+  proof.
+    by move=> h; apply big1_seq => i [] hP /mem_range hin; apply h.
+  qed.
+
+  lemma ex_CPA1_CPAn &m : 
+    exists (B <: AdvCPA [main : `{(cincr H.q + ceqint H.q + cltint H.q) * H.q + cdinterval H.q + (H.q - 1) * cs.`cenc + cA, 
+                                  #LR.orcl: 1}] 
+           {+A,+H.HybOrcl, +K, +S}),
+      (Pr[CPAL(S,A).main() @ &m : res] - Pr[CPAR(S,A).main() @ &m : res]) =
+      H.q%r * (Pr[CPAL(S,B).main() @ &m : res] - Pr[CPAR(S,B).main() @ &m : res]).
+  proof.
+    exists (B(S,A)); split; last by have -> := CPA1_CPAn &m; field; smt (H.q_pos).
+    move=> cLR MLR hcLR.
+    proc. 
+    seq 2 : (H.HybOrcl.l =0 /\ 0 <= H.HybOrcl.l0 < H.q) time [ (cincr H.q + ceqint H.q + cltint H.q) * H.q;
+                                                               S.enc : (H.q - 1);
+                                                               A.main : 1;
+                                                               MLR.orcl : 1].
+    + wp; rnd (0 <= H.q <= H.q - 0); skip => &hr />.
+      instantiate /(_ H.q) /= -> := (cost_dinterval {b' : bool, pk : pkey} 0 H.q).     
+      smt (DInterval.supp_dinter DInterval.dinter_ll H.q_pos).
+    exlim H.HybOrcl.l0 => l0. 
+    call (_: (0 <= H.HybOrcl.l /\ 0 <= H.HybOrcl.l0 <= H.q); 
+       (HybOrcl2(ToOrcl(S), MLR).orcl : H.HybOrcl.l) time
+      [ (HybOrcl2(ToOrcl(S), MLR).orcl : [fun _ => cincr H.q + ceqint H.q + cltint H.q ; S.enc : fun k => b2i (k <> l0); MLR.orcl : fun k => b2i(k=l0)]) ]) => //=.
+    + move=> zo hzo; proc; inline *; wp := (`|H.HybOrcl.l| <= H.q).
+      admit.
+      (* if := (`|H.HybOrcl.l| <= H.q). *)
+    skip => &hr />; move: (H.HybOrcl.l0{hr}) => {l0}l0 h0 hq .
+    rewrite bigi_constz 1:[smt (H.q_pos)] /=.
+    rewrite !big_b2i !(bigi_b2i_split l0 0 H.q) 1,2:// /b2i /=.
+    rewrite !(bigi_inP _ _ (fun (k : int) => k <> l0)) 1,2:/# !bigi_constz 1:// 1:/#.
+    by rewrite !bigi1 /= /#.
+  qed.
+  
+(* doute sur les borne  *)
+
+
+
+A(HybOrcl2(ToOrcl(S0), LR)
+print B.
+search (_ / _ = _)%Real.
+    
+    1%r/H.q%r * 
 
 end section.
